cedar-lean/Cedar/Thm/TPE/BatchedEvaluator.lean
@@ -29,7 +29,7 @@ in the code base at the moment.
 -/
 abbrev EntityLoader.WellBehaved (store: Entities) (loader: EntityLoader) : Prop :=
   ∀ s, s ⊆ (loader s).keys ∧
-       EntitiesRefine store ((loader s).mapOnValues EntityDataOption.asPartial)
+       EntitiesRefine store ((loader s).asPartial)
 
 theorem as_partial_request_refines {req : Request} :
   RequestRefines req (Request.asPartialRequest req) := by
@@ -51,27 +51,35 @@ theorem any_refines_empty_entities :
   intro a e₂ h₁
   contradiction
 
+theorem withMissing_asPartial_append {m1 m2 : EntitiesWithMissing} :
+  EntitiesWithMissing.asPartial (m1 ++ m2) = m1.asPartial ++ m2.asPartial := by
+  sorry
+
 -- Helper lemma for map append refinement
-theorem entities_refine_append (es : Entities) (m1 m2 : PartialEntities) :
-  EntitiesRefine es m1 → EntitiesRefine es m2 → EntitiesRefine es (m2 ++ m1) := by
+theorem entities_refine_withMissing_asPartial_append (es : Entities) (m2 m1 : EntitiesWithMissing) :
+  EntitiesRefine es m1.asPartial → EntitiesRefine es m2.asPartial → EntitiesRefine es (EntitiesWithMissing.asPartial (m1 ++ m2)) := by
   intro h1 h2
   unfold EntitiesRefine
   intro a e₂ h_find
+  rw [withMissing_asPartial_append] at h_find
+
   rw [Map.find?_append] at h_find
-  cases h_case : m2.find? a with
+  cases h_case : m1.find? a with
   | some e₂' =>
-    have h_eq : e₂ = e₂' := by
-      rw [h_case] at h_find
-      simp only [Option.some_or, Option.some.injEq] at h_find
-      rw [h_find]
+    unfold EntitiesWithMissing.asPartial at h_find
+    have h_find₂ : Map.find? m2.asPartial a = e₂'.asPartial := by
+      sorry
+    have h_eq : e₂ = e₂'.asPartial := by
+      sorry
     rw [h_eq]
-    exact h2 a e₂' h_case
+
+    exact h2 a e₂'.asPartial h_find₂
   | none =>
-    have h_find1 : m1.find? a = some e₂ := by
-      rw [h_case] at h_find
-      simp only [Option.none_or] at h_find
-      rw [h_find]
-    exact h1 a e₂ h_find1
+    have h_find₃ : m1.asPartial.find? a = none := by
+      sorry
+    have h_find₂ : m1.asPartial.find? a = some e₂ := by
+      sorry
+    exact h1 a e₂ h_find₂
 
 
 theorem direct_request_and_entities_refine (req : Request) (es : Entities) :
@@ -93,11 +101,11 @@ theorem batched_eval_loop_eq_evaluate
   {x : Residual}
   {req : Request}
   (es : Entities)
-  {current_store : PartialEntities}
+  {current_store : EntitiesWithMissing}
   {env : TypeEnv} :
   EntityLoader.WellBehaved es loader →
   Residual.WellTyped env x →
-  RequestAndEntitiesRefine req es req.asPartialRequest current_store →
+  RequestAndEntitiesRefine req es req.asPartialRequest current_store.asPartial →
   InstanceOfWellFormedEnvironment req es env →
   (Residual.evaluate (batchedEvalLoop x req loader current_store iters) req es).toOption = (Residual.evaluate x req es).toOption := by
   intro h₀ h₁ h₂ h₃
@@ -106,22 +114,23 @@ theorem batched_eval_loop_eq_evaluate
   case h_1 => simp only
   case h_2 iters n=>
     let toLoad := (Set.filter (fun uid => (Map.find? current_store uid).isNone) x.allLiteralUIDs)
-    let newEntities := ((loader toLoad).mapOnValues EntityDataOption.asPartial)
-    let newStore := newEntities ++ current_store
+    let newEntities := (loader toLoad)
+    let newStore: EntitiesWithMissing := newEntities ++ current_store
 
     have h₀₂ := h₀
     specialize h₀₂ toLoad
     obtain ⟨h₄, h₅⟩ := h₀₂
 
-    have h₆ : RequestAndEntitiesRefine req es req.asPartialRequest newStore := by
+    have h₆ : RequestAndEntitiesRefine req es req.asPartialRequest newStore.asPartial := by
       unfold RequestAndEntitiesRefine
       constructor
       · exact as_partial_request_refines
-      · apply entities_refine_append
-        · unfold RequestAndEntitiesRefine at h₂
-          exact h₂.right
-        · apply h₅
-    let newRes := TPE.evaluate x req.asPartialRequest newStore
+      · subst newStore
+        apply entities_refine_withMissing_asPartial_append
+        · exact h₅
+        · obtain ⟨_, h₂⟩ := h₂
+          exact h₂
+    let newRes := TPE.evaluate x req.asPartialRequest newStore.asPartial
     have h₇ : (Residual.evaluate newRes req es).toOption = (Residual.evaluate x req es).toOption := by
       subst newRes
       rw [← partial_evaluate_is_sound h₁ h₃ h₆]
